\begin{sol}
We want to show that $\bm{AB}=\bm{BA} \iff (\bm{A}+\bm{B})^2 = \bm{A}^2+2\bm{AB}+\bm{B^2}$. First we show that this holds backwards:
\begin{align}
    (\bm{A}+\bm{B})^2 &=     \bm{A}^2+\bm{AB}+\bm{AB}+\bm{B^2} & \text{(given)} \\ 
    \bm{A}^2+\bm{AB}+\bm{BA}+\bm{B^2} &= \bm{A}^2+\bm{AB}+\bm{AB}+\bm{B^2} \\
    \bm{BA} &= \bm{AB} & \text{(cancellation)}
\end{align}
Notice that the steps are reversible. We can explicitly complete the proof by working forwards. Assume $\bm{BA}=\bm{AB}$ is a given, then:
\begin{align}
    \bm{BA} &= \bm{AB} & \text{(given)} \\ 
    \bm{A}^2+\bm{AB}+\bm{BA}+\bm{B^2} &= \bm{A}^2+\bm{AB}+\bm{AB}+\bm{B^2} \\ 
    (\bm{A}+\bm{B})^2 &=     \bm{A}^2+2\bm{AB} +\bm{B^2} & \text{(factor)} 
\end{align}
\end{sol}