\begin{sol}
    From multilinearity, we have (using the first equality):
    \begin{equation}
        \frac{2^n}{\det \bff{A}} = -4 \implies \det \bff{A} = -2^{n-2}
    \end{equation}
    From the second set, applying the product rule, we have:
    \begin{equation}
        -4 = \frac{\det(\bff{A})^3}{\det \bff{B}}
    \end{equation}
    Since we know that $\det \bff{A} = -2^{n-2}$ we have:
    \begin{equation}
        -4 = \frac{-2^{3n-6}}{\det \bff{B}} \implies \det \bff{B} = 2^{3n-8}
    \end{equation}
\end{sol}