\begin{sol}
\begin{enumerate}[label=\textbf{(\alph*)}]
    \item Let $\bm{0} = (z_1,z_2)$. We want:
    \begin{align}
        (z_1,z_2) + (x_1,y_1) &= (x_1,y_1) \\ 
        (x_1+z_1+1, y_1+z_2+1) &= (x_1,y_1) 
    \end{align}
    The unique solution that accomplishes this is: $\bm{0} = (z_1,z_2) = (-1,-1)$.
    \item Let the additive inverse by $\bm{z}=(z_1,z_2)$. We want:
    \begin{align}
        (2,3) + (z_1,z_2) &= (-1,-1) \\ 
        (2+z_1+1,3+z_2+1) &= (-1,-1) 
    \end{align}
    We get the additive inverse to be:
    \begin{equation}
        -(2,3) = (-4,-5)
    \end{equation}
\end{enumerate}

\end{sol}