\begin{sol}
Let $\bm{0} = (z_1,z_2)$. We want:
    \begin{align}
        (z_1,z_2) + (x_1,y_1) &= (x_1,y_1) \\ 
        (x_1+z_1+k, y_1+z_2+k) &= (x_1,y_1)
    \end{align}
    The unique solution that accomplishes this is: $\bm{0} = (z_1,z_2) = (-k,-k)$.
 Let the additive inverse of $(x,y)$ $\bm{a}=(a_1,a_2)$. We want:
    \begin{align}
        (x,y) + (a_1,a_2) &= (-k,-k) \\ 
        (x+a_1+k,y+a_2+k) &= (-k,-k)
    \end{align}
    We get the additive inverse to be:
    \begin{equation}
       -(x,y) = (-x-2k,-y-2k)
    \end{equation}
\end{sol}