\section{Vector Spaces}
\begin{itemize}
    \item A vector space consistso f three things: a set $V$ together with the two operations of vector addition and scalar multiplication. We use $V$ to describe both the vector space and the set itself. Specifically:
    \begin{definition}
        A \textbf{real vector space} is a set $V$ together with two operations called \textit{vector addition} and \textit{scalar multiplication} such that the following \textit{axioms} hold:
        \vspace{2mm}
        \begin{enumerate}
            \setlength\itemsep{1em}
            \item \textbf{Additive Closure (AC):} For all vectors $\bm{x}, \bm{y} \in V$, $\bm{x}+\bm{y} \in V$.
            \item \textbf{Scalar Closure (SC):} For all vectors $\bm{x} \in V$, and scalars $c \in \mathbb{R}$, $c\bm{x} \in V$.
            \item \textbf{Additive Associativity (AA):} For all vectors $\bm{x},\bm{y},\bm{z} \in V$, $(\bm{x}+\bm{y})+\bm{z} = \bm{x} + (\bm{y}+\bm{z})$
            \item \textbf{Zero Vector (Z):} There exists a unique vector $\bm{0} \in V$ with the property that $\bm{x}+\bm{0}=\bm{x}$ for all vectors $\bm{x} \in V$.
            \item \textbf{Additive Inverse (AI):} For each vector $\bm{x} \in V$, there exists a unique vector $-\bm{x} \in V$ with the property that $\bm{x} + (-\bm{x})=\bm{0}$.
            \item \textbf{Scalar Multiplication Associativity (SMA):} For all vectors $\bm{x} \in V$, and scalars $c$, $d\in \mathbb{R}$, $(cd)\bm{x} = c(d\bm{x})$.
            \item \textbf{Distributivity of Vector Addition (DVA):} For all vectors $\bm{x},\bm{y} \in V$, and scalars $c \in \mathbb{R}$, $c(\bm{x}+\bm{y})=c\bm{x}+c\bm{y}$.
            \item \textbf{Distributivity of Scalar Addition (DSA):} For all vectors $\bm{x} \in V$, and scalars $c,d \in \mathbb{R}$, $(c+d)\bm{x}=c\bm{x}+d\bm{x}$.
            \item \textbf{Identity (I):} For all vectors $\bm{x} \in V$, $1\bm{x} = \bm{x}$.
        \end{enumerate}
    \end{definition}
    \item Note that \textit{anything} can be a vector space as long as we define operations such that it has properties that satisfies the above properties.
    \item To define a \textbf{complex vector space}, we let the scalars belong in the complex space instead.
    \begin{theorem}
        \textbf{The Cancellation Theorem:} Let $V$ be a vector space, and let $\bm{x}, \bm{y}, \bm{z} \in V$. If:
        \begin{equation}
            \bm{x}+ \bm{z} = \bm{y}+ \bm{z}
        \end{equation}
        then:
        \begin{equation}
            \bm{x} = \bm{y}
        \end{equation}
        \begin{proof}
            For $\bm{x},\bm{y},\bm{z} \in V$,
            \begin{align*}
                \bm{x} &= \bm{x} + \bm{0} & (Z) \\ 
                &= \bm{x} + (\bm{z} + -\bm{z}) & (AI) \\ 
                &= (\bm{x} + \bm{z}) + -\bm{z} & (AA) \\ 
                &= (\bm{y}+\bm{z}) + -\bm{z} & \text{(given)} \\
                &= \bm{y} + \bm{0} & (AI) \\ 
                &= \bm{y} & (Z)
            \end{align*}
            Alternatively:
            \begin{align*}
                \bm{x} + \bm{z} &= \bm{y} + \bm{z} & \text{(given)} \\ 
                \bm{x} + \bm{z} + -\bm{z} &= \bm{y} + \bm{z} + -\bm{z} \\ 
                \bm{x} + \bm{0} &= \bm{y} + \bm{0} & (AI) \\ 
                \bm{x} &= \bm{y} & (Z)
            \end{align*}
        \end{proof}
    \end{theorem}
    \begin{proposition}
        Let $V$ be a vector space and let $\bm{x} \in V$. Then $0\bm{x} = \bm{0}$.
        \begin{proof}
            For $\bm{x} \in V$:
            \begin{align*}
                0\bm{x} &= (0+0)\bm{x} \\ 
                &= 0\bm{x} + 0\bm{x} & (DSA) \\ 
                0\bm{x} + -0\bm{x} &= 0\bm{x} + 0\bm{x} + -0\bm{x} \\ 
                \bm{0} &= 0\bm{x} + \bm{0} & (AI) \\ 
                \bm{0} &= 0\bm{x} & (Z)
            \end{align*}
        \end{proof}
    \end{proposition}
    \begin{proposition}
        Let $V$ be a vector space, and let $\bm{x} \in V$. Then $(-1)\bm{x}=-\bm{x}$.
        \begin{proof}
            For $\bm{x} \in V$,
            \begin{align*}
                -\bm{x} = -\bm{x} + \bm{0} & (Z) \\ 
                &= -\bm{x} + 0\bm{x} & (P1) \\ 
                &= -\bm{x} + (1 + (-1))\bm{x} \\ 
                &= -\bm{x}+1\bm{x}+(-1)\bm{x} & (DSA) \\ 
                &= (-\bm{x}+\bm{x}) + (-1)\bm{x} & (AA) \\ 
                &= \bm{0} + (-1)\bm{x} & (P3) \\ 
                &= (-1)\bm{x} & (P4)
            \end{align*}
        \end{proof}
    \end{proposition}
    \begin{proposition}
        Let $V$ be a vector space and let $\bm{x} \in V$. Then $-\bm{x}+\bm{x}=\bm{0}$.
        \begin{proof}
            For $x \in V$,
            \begin{align*}
                -\bm{x}+\bm{x} &= -\bm{x}+\bm{x} + \bm{0} & (Z) \\ 
                &= -\bm{x}+\bm{x}+\left((-\bm{x}+\bm{x})+-(\bm{-x}+\bm{x})\right) & (AI) \\ 
                &= ((-\bm{x}+\bm{x})+(-\bm{x}+\bm{x}))+-(-\bm{x}+\bm{x}) & (AA) \\ 
                &= (-\bm{x}+(\bm{x}+(-\bm{x}+\bm{x}))) +-(-\bm{x}+\bm{x}) & (AA) \\ 
                &= (-\bm{x}+((\bm{x}+-\bm{x})+\bm{x}))+-(-\bm{x}+\bm{x}) & (AA) \\ 
                &= (-\bm{x}+(\bm{0} + \bm{x})) +-(-\bm{x}+\bm{x}) & (Z) \\ 
                &= ((-\bm{x}+\bm{0})+\bm{x})) + -(-\bm{x}+\bm{x}) & (AI) \\
                &=  (-\bm{x}+\bm{x})+-(-\bm{x}+\bm{x})  & (Z) \\ 
                &= \bm{0} & (AI)
            \end{align*}
        \end{proof}
    \end{proposition}
    \begin{proposition}
        Let $V$ be a vector space, and let $\bm{x}\in V$. Then $\bm{0}+\bm{x}=\bm{x}$.
        \begin{proof}
            For $x\in V$,
            \begin{align*}
                \bm{0} + \bm{x} &= (\bm{x}+(-\bm{x}))+ \bm{x} & (AI) \\ 
                &= \bm{x} + (-\bm{x} + \bm{x}) & (AA) \\ 
                &= \bm{x} + \bm{0} & (P3) \\
                &= \bm{x} & (Z)
            \end{align*}
        \end{proof}
    \end{proposition}
\end{itemize}